update

04_Earley_Recognizer.thy
@@ -7,31 +7,6 @@ begin
 
 chapter\<open>Earley Recognizer Implementation \label{chap:04}\<close> 
 
-section \<open>Draft\<close>
-
-text\<open>
-  \begin{itemize}
-    \item introduce auxiliary definitions: filter\_with\_index, pointer, entry in more detail
-      most everything else in text
-    \item overview over earley implementation with linked list and pointers and the mapping into a
-      functional setting
-    \item introduce Init\_it, Scan\_it, Predict\_it and Complete\_it, compare them with the set notation
-      and discuss performance improvements (Grammar in more specific form) Why do they all return a list?!
-    \item discus bin(s)\_upd(s) functions. Why bin\_upds like this -> easier than fold for proofs!
-    \item discuss pi\_it and why it is a partial function -> only terminates for valid input and foreshadow
-      how this is done in isabelle
-    \item introduce remaining definitions (analog to sets)
-    \item discuss wf proofs quickly and go into detail about isabelle specifics about termination and
-      the custom induction scheme using finiteness
-    \item outline the approach to proof correctness aka subsumption in both directions
-    \item discuss list to set proofs
-    \item discuss soundness proofs (maybe omit since obvious)
-    \item discuss completeness proof focusing on the complete case shortly explaining scan and predict
-      which don't change via iteration and order does not matter
-    \item highlight main theorems
-  \end{itemize}
-\<close>
-
 text\<open>
   \begin{table}[htpb]
     \caption[Earley items with pointers running example]{Earley items with pointers for the grammar @{term \<G>}: $S \rightarrow \, x$, $S \rightarrow \, S + S$}\label{tab:earley-items}
@@ -78,9 +53,6 @@ definition items :: "'a bin \<Rightarrow> 'a item list" where
 definition pointers :: "'a bin \<Rightarrow> pointer list" where
   "pointers b = map pointer b"
 
-definition bins_eq_items :: "'a bins \<Rightarrow> 'a bins \<Rightarrow> bool" where
-  "bins_eq_items bs0 bs1 \<longleftrightarrow> map items bs0 = map items bs1"
-
 definition bins_items :: "'a bins \<Rightarrow> 'a items" where
   "bins_items bs = \<Union> { set (items (bs!k)) | k. k < length bs }"
 
@@ -88,30 +60,30 @@ definition bin_items_upto :: "'a bin \<Rightarrow> nat \<Rightarrow> 'a items" w
   "bin_items_upto b i = { items b ! j | j. j < i \<and> j < length (items b) }"
 
 definition bins_items_upto :: "'a bins \<Rightarrow> nat \<Rightarrow> nat \<Rightarrow> 'a items" where
-  "bins_items_upto bs k i = \<Union> { set (items (bs ! l)) | l. l < k } \<union> bin_items_upto (bs ! k) i"
+  "bins_items_upto bs k i = \<Union> { set (items (bs!l)) | l. l < k } \<union> bin_items_upto (bs!k) i"
 
 definition wf_bin_items :: "'a cfg \<Rightarrow> 'a sentential \<Rightarrow> nat \<Rightarrow> 'a item list \<Rightarrow> bool" where
-  "wf_bin_items cfg inp k xs \<equiv> \<forall>x \<in> set xs. wf_item cfg inp x \<and> item_end x = k"
+  "wf_bin_items cfg \<omega> k xs \<equiv> \<forall>x \<in> set xs. wf_item cfg \<omega> x \<and> item_end x = k"
 
 definition wf_bin :: "'a cfg \<Rightarrow> 'a sentential \<Rightarrow> nat \<Rightarrow> 'a bin \<Rightarrow> bool" where
-  "wf_bin cfg inp k b \<equiv> distinct (items b) \<and> wf_bin_items cfg inp k (items b)"
+  "wf_bin cfg \<omega> k b \<equiv> distinct (items b) \<and> wf_bin_items cfg \<omega> k (items b)"
 
 definition wf_bins :: "'a cfg \<Rightarrow> 'a list \<Rightarrow> 'a bins \<Rightarrow> bool" where
-  "wf_bins cfg inp bs \<equiv> \<forall>k < length bs. wf_bin cfg inp k (bs ! k)"
+  "wf_bins cfg \<omega> bs \<equiv> \<forall>k < length bs. wf_bin cfg \<omega> k (bs!k)"
 
 definition nonempty_derives :: "'a cfg \<Rightarrow> bool" where
   "nonempty_derives cfg \<equiv> \<forall>N. N \<in> set (\<NN> cfg) \<longrightarrow> \<not> derives cfg [N] []"
 
 definition Init_list :: "'a cfg \<Rightarrow> 'a sentential \<Rightarrow> 'a bins" where
-  "Init_list cfg inp \<equiv> 
+  "Init_list cfg \<omega> \<equiv> 
     let rs = filter (\<lambda>r. rule_head r = \<SS> cfg) (\<RR> cfg) in
     let b0 = map (\<lambda>r. (Entry (init_item r 0) Null)) rs in
-    let bs = replicate (length inp + 1) ([]) in
+    let bs = replicate (length \<omega> + 1) ([]) in
     bs[0 := b0]"
 
 definition Scan_list :: "nat \<Rightarrow> 'a sentential \<Rightarrow> 'a  \<Rightarrow> 'a item \<Rightarrow> nat \<Rightarrow> 'a entry list" where
-  "Scan_list k inp a x pre \<equiv>
-    if inp!k = a then
+  "Scan_list k \<omega> a x pre \<equiv>
+    if \<omega>!k = a then
       let x' = inc_item x (k+1) in
       [Entry x' (Pre pre)]
     else []"
@@ -155,152 +127,80 @@ definition bins_upd :: "'a bins \<Rightarrow> nat \<Rightarrow> 'a entry list \<
   "bins_upd bs k es = bs[k := bin_upds es (bs!k)]"
 
 partial_function (tailrec) Earley_bin_list' :: "nat \<Rightarrow> 'a cfg \<Rightarrow> 'a sentential \<Rightarrow> 'a bins \<Rightarrow> nat \<Rightarrow> 'a bins" where
-  "Earley_bin_list' k cfg inp bs i = (
-    if i \<ge> length (items (bs ! k)) then bs
+  "Earley_bin_list' k cfg \<omega> bs i = (
+    if i \<ge> length (items (bs!k)) then bs
     else
       let x = items (bs!k) ! i in
       let bs' =
         case next_symbol x of
           Some a \<Rightarrow>
             if is_terminal cfg a then
-              if k < length inp then bins_upd bs (k+1) (Scan_list k inp a x i)
+              if k < length \<omega> then bins_upd bs (k+1) (Scan_list k \<omega> a x i)
               else bs
             else bins_upd bs k (Predict_list k cfg a)
         | None \<Rightarrow> bins_upd bs k (Complete_list k x bs i)
-      in Earley_bin_list' k cfg inp bs' (i+1))"
+      in Earley_bin_list' k cfg \<omega> bs' (i+1))"
 
 definition Earley_bin_list :: "nat \<Rightarrow> 'a cfg \<Rightarrow> 'a sentential \<Rightarrow> 'a bins \<Rightarrow> 'a bins" where
-  "Earley_bin_list k cfg inp bs = Earley_bin_list' k cfg inp bs 0"
+  "Earley_bin_list k cfg \<omega> bs = Earley_bin_list' k cfg \<omega> bs 0"
 
 fun Earley_list :: "nat \<Rightarrow> 'a cfg \<Rightarrow> 'a sentential \<Rightarrow> 'a bins" where
-  "Earley_list 0 cfg inp = Earley_bin_list 0 cfg inp (Init_list cfg inp)"
-| "Earley_list (Suc n) cfg inp = Earley_bin_list (Suc n) cfg inp (Earley_list n cfg inp)"
+  "Earley_list 0 cfg \<omega> = Earley_bin_list 0 cfg \<omega> (Init_list cfg \<omega>)"
+| "Earley_list (Suc n) cfg \<omega> = Earley_bin_list (Suc n) cfg \<omega> (Earley_list n cfg \<omega>)"
 
 definition \<E>arley_list :: "'a cfg \<Rightarrow> 'a sentential \<Rightarrow> 'a bins" where
-  "\<E>arley_list cfg inp = Earley_list (length inp) cfg inp"
+  "\<E>arley_list cfg \<omega> = Earley_list (length \<omega>) cfg \<omega>"
+
+section \<open>Sets or bins as list\<close>
+
+lemma set_items_bin_upd:
+  "set (items (bin_upd e b)) = set (items b) \<union> {item e}"
+(*<*)
+  sorry
+(*>*)
+
+text\<open>\<close>
+
+lemma set_items_bin_upds:
+  "set (items (bin_upds es b)) = set (items b) \<union> set (items es)"
+(*<*)
+  sorry
+(*>*)
+
+text\<open>\<close>
+
+lemma bins_items_bins_upd:
+  assumes "k < length bs"
+  shows "bins_items (bins_upd bs k es) = bins_items bs \<union> set (items es)"
+(*<*)
+  sorry
+(*>*)
+
+text\<open>Similar lemmas about @{term bins_items_upto}\<close>
 
 section \<open>Wellformedness\<close>
 
-lemma wf_bin_bin_upd:
-  assumes "wf_bin cfg inp k b" "wf_item cfg inp (item e)" "item_end (item e) = k"
-  shows "wf_bin cfg inp k (bin_upd e b)"
-(*<*)
-  sorry
-(*>*)
+text\<open>Just note that @{term bin_upd}, @{term bin_upds}, @{term bins_upd}, @{term Init_list},
+@{term Scan_list}, @{term Predict_list}, @{term Complete_list} only generate @{term wf_bin} or
+@{term wf_bins}\<close>
 
-text\<open>\<close>
-
-lemma wf_bin_bin_upds:
-  assumes "wf_bin cfg inp k b" "distinct (items es)"
-  assumes "\<forall>x \<in> set (items es). wf_item cfg inp x \<and> item_end x = k"
-  shows "wf_bin cfg inp k (bin_upds es b)"
-(*<*)
-  sorry
-(*>*)
-
-text\<open>\<close>
-
-lemma wf_bins_bins_upd:
-  assumes "wf_bins cfg inp bs" "distinct (items es)"
-  assumes "\<forall>x \<in> set (items es). wf_item cfg inp x \<and> item_end x = k"
-  shows "wf_bins cfg inp (bins_upd bs k es)"
-(*<*)
-  sorry
-(*>*)
-
-text\<open>\<close>
-
-lemma wf_bins_Init_list:
-  assumes "wf_cfg cfg"
-  shows "wf_bins cfg inp (Init_list cfg inp)"
-(*<*)
-  sorry
-(*>*)
-
-text\<open>\<close>
-
-lemma wf_bins_Scan_list:
-  assumes "wf_bins cfg inp bs" "k < length bs" "x \<in> set (items (bs!k))" "k < length inp" "next_symbol x \<noteq> None"
-  shows "\<forall>y \<in> set (items (Scan_list k inp a x pre)). wf_item cfg inp y \<and> item_end y = k+1"
-(*<*)
-  sorry
-(*>*)
-
-text\<open>\<close>
-
-lemma wf_bins_Predict_list:
-  assumes "wf_bins cfg inp bs" "k < length bs" "k \<le> length inp" "wf_cfg cfg"
-  shows "\<forall>y \<in> set (items (Predict_list k cfg X)). wf_item cfg inp y \<and> item_end y = k"
-(*<*)
-  sorry
-(*>*)
-
-text\<open>\<close>
-
-lemma wf_bins_Complete_list:
-  assumes "wf_bins cfg inp bs" "k < length bs" "y \<in> set (items (bs!k))"
-  shows "\<forall>x \<in> set (items (Complete_list k y bs red)). wf_item cfg inp x \<and> item_end x = k"
-(*<*)
-  sorry
-(*>*)
-
-text\<open>\<close>
+text\<open>Explain termination, how it is proved in Isabelle and custom induction schema.\<close>
 
 fun earley_measure :: "nat \<times> 'a cfg \<times> 'a sentential \<times> 'a bins \<Rightarrow> nat \<Rightarrow> nat" where
-  "earley_measure (k, cfg, inp, bs) i = card { x | x. wf_item cfg inp x \<and> item_end x = k } - i"
+  "earley_measure (k, cfg, \<omega>, bs) i = card { x | x. wf_item cfg \<omega> x \<and> item_end x = k } - i"
 
 definition wf_earley_input :: "(nat \<times> 'a cfg \<times> 'a sentential \<times> 'a bins) set" where
   "wf_earley_input = { 
-    (k, cfg, inp, bs) | k cfg inp bs.
-      k \<le> length inp \<and>
-      length bs = length inp + 1 \<and>
+    (k, cfg, \<omega>, bs) | k cfg \<omega> bs.
+      k \<le> length \<omega> \<and>
+      length bs = length \<omega> + 1 \<and>
       wf_cfg cfg \<and>
-      wf_bins cfg inp bs
+      wf_bins cfg \<omega> bs
   }"
 
-lemma wf_earley_input_Init_list:
-  assumes "k \<le> length inp" "wf_cfg cfg"
-  shows "(k, cfg, inp, Init_list cfg inp) \<in> wf_earley_input"
-(*<*)
-  sorry
-(*>*)
-
-text\<open>\<close>
-
-lemma wf_earley_input_Complete_list:
-  assumes "(k, cfg, inp, bs) \<in> wf_earley_input" "\<not> length (items (bs!k)) \<le> i"
-  assumes "x = items (bs!k)!i" "next_symbol x = None"
-  shows "(k, cfg, inp, bins_upd bs k (Complete_list k x bs red)) \<in> wf_earley_input"
-(*<*)
-  sorry
-(*>*)
-
-text\<open>\<close>
-
-lemma wf_earley_input_Scan_list:
-  assumes "(k, cfg, inp, bs) \<in> wf_earley_input" "\<not> length (items (bs!k)) \<le> i"
-  assumes "x = items (bs!k)!i" "next_symbol x = Some a"
-  assumes "is_terminal cfg a" "k < length inp"
-  shows "(k, cfg, inp, bins_upd bs (k+1) (Scan_list k inp a x pre)) \<in> wf_earley_input"
-(*<*)
-  sorry
-(*>*)
-
-text\<open>\<close>
-
-lemma wf_earley_input_Predict_list:
-  assumes "(k, cfg, inp, bs) \<in> wf_earley_input" "\<not> length (items (bs!k)) \<le> i"
-  assumes "x = items (bs!k)!i" "next_symbol x = Some a" "\<not> is_terminal cfg a"
-  shows "(k, cfg, inp, bins_upd bs k (Predict_list k cfg a)) \<in> wf_earley_input"
-(*<*)
-  sorry
-(*>*)
-
-text\<open>\<close>
-
 lemma wf_earley_input_Earley_bin_list':
-  assumes "(k, cfg, inp, bs) \<in> wf_earley_input" 
-  shows "(k, cfg, inp, Earley_bin_list' k cfg inp bs i) \<in> wf_earley_input"
+  assumes "(k, cfg, \<omega>, bs) \<in> wf_earley_input" 
+  shows "(k, cfg, \<omega>, Earley_bin_list' k cfg \<omega> bs i) \<in> wf_earley_input"
 (*<*)
   sorry
 (*>*)
@@ -308,8 +208,8 @@ lemma wf_earley_input_Earley_bin_list':
 text\<open>\<close>
 
 lemma wf_earley_input_Earley_bin_list:
-  assumes "(k, cfg, inp, bs) \<in> wf_earley_input" 
-  shows "(k, cfg, inp, Earley_bin_list k cfg inp bs) \<in> wf_earley_input"
+  assumes "(k, cfg, \<omega>, bs) \<in> wf_earley_input" 
+  shows "(k, cfg, \<omega>, Earley_bin_list k cfg \<omega> bs) \<in> wf_earley_input"
 (*<*)
   sorry
 (*>*)
@@ -317,8 +217,9 @@ lemma wf_earley_input_Earley_bin_list:
 text\<open>\<close>
 
 lemma wf_earley_input_Earley_list:
-  assumes "k \<le> length inp" "wf_cfg cfg"
-  shows "(k, cfg, inp, Earley_list k cfg inp) \<in> wf_earley_input"
+  assumes "wf_cfg cfg"
+  assumes "k \<le> length \<omega>"
+  shows "(k, cfg, \<omega>, Earley_list k cfg \<omega>) \<in> wf_earley_input"
 (*<*)
   sorry
 (*>*)
@@ -326,44 +227,9 @@ lemma wf_earley_input_Earley_list:
 text\<open>\<close>
 
 lemma wf_earley_input_\<E>arley_list:
-  assumes "k \<le> length inp" "wf_cfg cfg"
-  shows "(k, cfg, inp, \<E>arley_list cfg inp) \<in> wf_earley_input"
-(*<*)
-  sorry
-(*>*)
-
-text\<open>\<close>
-
-lemma wf_bins_Earley_bin_list':
-  assumes "(k, cfg, inp, bs) \<in> wf_earley_input" 
-  shows "wf_bins cfg inp (Earley_bin_list' k cfg inp bs i)"
-(*<*)
-  sorry
-(*>*)
-
-text\<open>\<close>
-
-lemma wf_bins_Earley_bin_list:
-  assumes "(k, cfg, inp, bs) \<in> wf_earley_input" 
-  shows "wf_bins cfg inp (Earley_bin_list k cfg inp bs)"
-(*<*)
-  sorry
-(*>*)
-
-text\<open>\<close>
-
-lemma wf_bins_Earley_list:
-  assumes "k \<le> length inp" "wf_cfg cfg"
-  shows "wf_bins cfg inp (Earley_list k cfg inp)"
-(*<*)
-  sorry
-(*>*)
-
-text\<open>\<close>
-
-lemma wf_bins_\<E>arley_list:
-  assumes "wf_cfg cfg" 
-  shows "wf_bins cfg inp (\<E>arley_list cfg inp)"
+  assumes "wf_cfg cfg"
+  assumes "k \<le> length \<omega>"
+  shows "(k, cfg, \<omega>, \<E>arley_list cfg \<omega>) \<in> wf_earley_input"
 (*<*)
   sorry
 (*>*)
@@ -371,7 +237,7 @@ lemma wf_bins_\<E>arley_list:
 section \<open>Soundness\<close>
 
 lemma Init_list_eq_Init:
-  shows "bins_items (Init_list cfg inp) = Init cfg"
+  shows "bins_items (Init_list cfg \<omega>) = Init cfg"
 (*<*)
   sorry
 (*>*)
@@ -379,9 +245,13 @@ lemma Init_list_eq_Init:
 text\<open>\<close>
 
 lemma Scan_list_sub_Scan:
-  assumes "wf_bins cfg inp bs" "bins_items bs \<subseteq> I" "x \<in> set (items (bs ! k))"
-  assumes "k < length bs" "k < length inp" "next_symbol x = Some a"
-  shows "set (items (Scan_list k inp a x pre)) \<subseteq> Scan k inp I"
+  assumes "wf_bins cfg \<omega> bs"
+  assumes "bins_items bs \<subseteq> I"
+  assumes "k < length bs"
+  assumes "k < length \<omega>"
+  assumes "x \<in> set (items (bs!k))"
+  assumes "next_symbol x = Some a"
+  shows "set (items (Scan_list k \<omega> a x pre)) \<subseteq> Scan k \<omega> I"
 (*<*)
   sorry
 (*>*)
@@ -389,7 +259,10 @@ lemma Scan_list_sub_Scan:
 text\<open>\<close>
 
 lemma Predict_list_sub_Predict:
-  assumes "wf_bins cfg inp bs" "bins_items bs \<subseteq> I" "x \<in> set (items (bs ! k))" "k < length bs"
+  assumes "wf_bins cfg \<omega> bs"
+  assumes "bins_items bs \<subseteq> I"
+  assumes "k < length bs"
+  assumes "x \<in> set (items (bs!k))"
   assumes "next_symbol x = Some X"
   shows "set (items (Predict_list k cfg X)) \<subseteq> Predict k cfg I"
 (*<*)
@@ -399,29 +272,32 @@ lemma Predict_list_sub_Predict:
 text\<open>\<close>
 
 lemma Complete_list_sub_Complete:
-  assumes "wf_bins cfg inp bs" "bins_items bs \<subseteq> I" "y \<in> set (items (bs ! k))" "k < length bs"
-  assumes "next_symbol y = None"
-  shows "set (items (Complete_list k y bs red)) \<subseteq> Complete k I"
+  assumes "wf_bins cfg \<omega> bs"
+  assumes "bins_items bs \<subseteq> I"
+  assumes "k < length bs"
+  assumes "x \<in> set (items (bs!k))"
+  assumes "next_symbol x = None"
+  shows "set (items (Complete_list k x bs red)) \<subseteq> Complete k I"
 (*<*)
   sorry
 (*>*)
 
 text\<open>\<close>
 
-lemma Earley_bin_list'_sub_E:
-  assumes "(k, cfg, inp, bs) \<in> wf_earley_input"
+lemma Earley_bin_list'_sub_Earley_bin:
+  assumes "(k, cfg, \<omega>, bs) \<in> wf_earley_input"
   assumes "bins_items bs \<subseteq> I"
-  shows "bins_items (Earley_bin_list' k cfg inp bs i) \<subseteq> E k cfg inp I"
+  shows "bins_items (Earley_bin_list' k cfg \<omega> bs i) \<subseteq> Earley_bin k cfg \<omega> I"
 (*<*)
   sorry
 (*>*)
 
 text\<open>\<close>
 
-lemma Earley_bin_list_sub_E:
-  assumes "(k, cfg, inp, bs) \<in> wf_earley_input"
+lemma Earley_bin_list_sub_Earley_bin:
+  assumes "(k, cfg, \<omega>, bs) \<in> wf_earley_input"
   assumes "bins_items bs \<subseteq> I"
-  shows "bins_items (Earley_bin_list k cfg inp bs) \<subseteq> E k cfg inp I"
+  shows "bins_items (Earley_bin_list k cfg \<omega> bs) \<subseteq> Earley_bin k cfg \<omega> I"
 (*<*)
   sorry
 (*>*)
@@ -429,26 +305,32 @@ lemma Earley_bin_list_sub_E:
 text\<open>\<close>
 
 lemma Earley_list_sub_\<E>:
-  assumes "k \<le> length inp" "wf_cfg cfg"
-  shows "bins_items (Earley_list k cfg inp) \<subseteq> \<E> k cfg inp"
+  assumes "wf_cfg cfg"
+  assumes "k \<le> length \<omega>"
+  shows "bins_items (Earley_list k cfg \<omega>) \<subseteq> Earley k cfg \<omega>"
 (*<*)
   sorry
 (*>*)
 
 text\<open>\<close>
 
-lemma \<E>arley_list_sub_earley:
+lemma \<E>arley_list_sub_\<E>arley:
   assumes "wf_cfg cfg" 
-  shows "bins_items (\<E>arley_list cfg inp) \<subseteq> earley cfg inp"
+  shows "bins_items (\<E>arley_list cfg \<omega>) \<subseteq> \<E>arley cfg \<omega>"
 (*<*)
   sorry
 (*>*)
 
 section \<open>Completeness\<close>
 
-lemma impossible_complete_item:
-  assumes "wf_cfg cfg" "wf_item cfg inp x" "sound_item cfg inp x"
-  assumes "is_complete x"  "item_origin x = k" "item_end x = k" "nonempty_derives cfg"
+lemma impossible_complete_item: \<comment>\<open>Detailed\<close>
+  assumes "wf_cfg cfg"
+  assumes "nonempty_derives cfg"
+  assumes "wf_item cfg \<omega> x"
+  assumes "sound_item cfg \<omega> x"
+  assumes "is_complete x" 
+  assumes "item_origin x = k"
+  assumes "item_end x = k"
   shows False
 (*<*)
   sorry
@@ -456,79 +338,89 @@ lemma impossible_complete_item:
 
 text\<open>\<close>
 
-lemma Complete_Un_eq_terminal:
-  assumes "next_symbol z = Some a" "is_terminal cfg a" "wf_items cfg inp I" "wf_item cfg inp z" "wf_cfg cfg"
-  shows "Complete k (I \<union> {z}) = Complete k I"
+lemma Complete_Un_eq_terminal: \<comment>\<open>Detailed?\<close>
+  assumes "wf_cfg cfg"
+  assumes "wf_items cfg \<omega> I"
+  assumes "wf_item cfg \<omega> x"
+  assumes "next_symbol z = Some a"
+  assumes "is_terminal cfg a"
+  shows "Complete k (I \<union> {x}) = Complete k I"
 (*<*)
   sorry
 (*>*)
 
 text\<open>\<close>
 
-lemma Complete_Un_eq_nonterminal:
-  assumes "next_symbol z = Some a" "is_nonterminal cfg a" "sound_items cfg inp I" "item_end z = k"
-  assumes "wf_items cfg inp I" "wf_item cfg inp z" "wf_cfg cfg" "nonempty_derives cfg"
-  shows "Complete k (I \<union> {z}) = Complete k I"
+lemma Complete_Un_eq_nonterminal: \<comment>\<open>Detailed?\<close>
+  assumes "wf_cfg cfg"
+  assumes "wf_items cfg \<omega> I"
+  assumes "sound_items cfg \<omega> I"
+  assumes "nonempty_derives cfg"
+  assumes "wf_item cfg \<omega> x"
+  assumes "item_end x = k"
+  assumes "next_symbol z = Some a"
+  assumes "is_nonterminal cfg a"
+  shows "Complete k (I \<union> {x}) = Complete k I"
 (*<*)
   sorry
 (*>*)
 
 text\<open>\<close>
 
-lemma Complete_sub_bins_Un_Complete_list:
-  assumes "Complete k I \<subseteq> bins_items bs" "I \<subseteq> bins_items bs" "is_complete z" "wf_bins cfg inp bs" "wf_item cfg inp z"
-  shows "Complete k (I \<union> {z}) \<subseteq> bins_items bs \<union> set (items (Complete_list k z bs red))"
+lemma Complete_sub_bins_Un_Complete_list: \<comment>\<open>Detailed?\<close>
+  assumes "wf_bins cfg \<omega> bs"
+  assumes "wf_item cfg \<omega> x"
+  assumes "is_complete z"
+  assumes "Complete k I \<subseteq> bins_items bs"
+  assumes "I \<subseteq> bins_items bs"
+  shows "Complete k (I \<union> {x}) \<subseteq> bins_items bs \<union> set (items (Complete_list k x bs red))"
 (*<*)
   sorry
 (*>*)
 
 text\<open>\<close>
 
-lemma Earley_bin_list'_mono:
-  assumes "(k, cfg, inp, bs) \<in> wf_earley_input"
-  shows "bins_items bs \<subseteq> bins_items (Earley_bin_list' k cfg inp bs i)"
+lemma Earley_bin_list'_mono: \<comment>\<open>Omit?\<close>
+  assumes "(k, cfg, \<omega>, bs) \<in> wf_earley_input"
+  shows "bins_items bs \<subseteq> bins_items (Earley_bin_list' k cfg \<omega> bs i)"
 (*<*)
   sorry
 (*>*)
 
 text\<open>\<close>
 
-lemma E_step_sub_Earley_bin_list':
-  assumes "(k, cfg, inp, bs) \<in> wf_earley_input"
-  assumes "E_step k cfg inp (bins_items_upto bs k i) \<subseteq> bins_items bs"
-  assumes "sound_items cfg inp (bins_items bs)" "is_sentence cfg inp" "nonempty_derives cfg"
-  shows "E_step k cfg inp (bins_items bs) \<subseteq> bins_items (Earley_bin_list' k cfg inp bs i)"
+lemma Earley_step_sub_Earley_bin_list': \<comment>\<open>Detailed: START WITH THIS\<close>
+  assumes "(k, cfg, \<omega>, bs) \<in> wf_earley_input"
+  assumes "sound_items cfg \<omega> (bins_items bs)"
+  assumes "is_sentence cfg \<omega>"
+  assumes "nonempty_derives cfg"
+  assumes "Earley_step k cfg \<omega> (bins_items_upto bs k i) \<subseteq> bins_items bs"
+  shows "Earley_step k cfg \<omega> (bins_items bs) \<subseteq> bins_items (Earley_bin_list' k cfg \<omega> bs i)"
 (*<*)
   sorry
 (*>*)
 
 text\<open>\<close>
 
-lemma E_step_sub_Earley_bin_list:
-  assumes "(k, cfg, inp, bs) \<in> wf_earley_input"
-  assumes "E_step k cfg inp (bins_items_upto bs k 0) \<subseteq> bins_items bs"
-  assumes "sound_items cfg inp (bins_items bs)" "is_sentence cfg inp" "nonempty_derives cfg"
-  shows "E_step k cfg inp (bins_items bs) \<subseteq> bins_items (Earley_bin_list k cfg inp bs)"
+lemma Earley_step_sub_Earley_bin_list:
+  assumes "(k, cfg, \<omega>, bs) \<in> wf_earley_input"
+  assumes "sound_items cfg \<omega> (bins_items bs)"
+  assumes "is_sentence cfg \<omega>"
+  assumes "nonempty_derives cfg"
+  assumes "Earley_step k cfg \<omega> (bins_items_upto bs k 0) \<subseteq> bins_items bs"
+  shows "Earley_step k cfg \<omega> (bins_items bs) \<subseteq> bins_items (Earley_bin_list k cfg \<omega> bs)"
 (*<*)
   sorry
 (*>*)
 
 text\<open>\<close>
 
-lemma Earley_bin_list'_bins_items_eq:
-  assumes "(k, cfg, inp, as) \<in> wf_earley_input"
-  assumes "bins_eq_items as bs" "wf_bins cfg inp as"
-  shows "bins_eq_items (Earley_bin_list' k cfg inp as i) (Earley_bin_list' k cfg inp bs i)"
-(*<*)
-  sorry
-(*>*)
-
-text\<open>\<close>
-
-lemma Earley_bin_list'_idem:
-  assumes "(k, cfg, inp, bs) \<in> wf_earley_input"
-  assumes "i \<le> j" "sound_items cfg inp (bins_items bs)" "nonempty_derives cfg"
-  shows "bins_items (Earley_bin_list' k cfg inp (Earley_bin_list' k cfg inp bs i) j) = bins_items (Earley_bin_list' k cfg inp bs i)"
+lemma Earley_bin_list'_idem: \<comment>\<open>Detailed: SECOND IS THIS\<close>
+  assumes "(k, cfg, \<omega>, bs) \<in> wf_earley_input"
+  assumes "sound_items cfg \<omega> (bins_items bs)"
+  assumes "nonempty_derives cfg"
+  assumes "i \<le> j"
+  shows "bins_items (Earley_bin_list' k cfg \<omega> (Earley_bin_list' k cfg \<omega> bs i) j) = bins_items (Earley_bin_list' k cfg \<omega> bs i)"
 (*<*)
   sorry
 (*>*)
@@ -536,31 +428,23 @@ lemma Earley_bin_list'_idem:
 text\<open>\<close>
 
 lemma Earley_bin_list_idem:
-  assumes "(k, cfg, inp, bs) \<in> wf_earley_input"
-  assumes "sound_items cfg inp (bins_items bs)" "nonempty_derives cfg"
-  shows "bins_items (Earley_bin_list k cfg inp (Earley_bin_list k cfg inp bs)) = bins_items (Earley_bin_list k cfg inp bs)"
+  assumes "(k, cfg, \<omega>, bs) \<in> wf_earley_input"
+  assumes "sound_items cfg \<omega> (bins_items bs)"
+  assumes "nonempty_derives cfg"
+  shows "bins_items (Earley_bin_list k cfg \<omega> (Earley_bin_list k cfg \<omega> bs)) = bins_items (Earley_bin_list k cfg \<omega> bs)"
 (*<*)
   sorry
 (*>*)
 
 text\<open>\<close>
 
-lemma funpower_E_step_sub_Earley_bin_list:
-  assumes "(k, cfg, inp, bs) \<in> wf_earley_input"
-  assumes "E_step k cfg inp (bins_items_upto bs k 0) \<subseteq> bins_items bs" "sound_items cfg inp (bins_items bs)"
-  assumes "is_sentence cfg inp" "nonempty_derives cfg"
-  shows "funpower (E_step k cfg inp) n (bins_items bs) \<subseteq> bins_items (Earley_bin_list k cfg inp bs)"
-(*<*)
-  sorry
-(*>*)
-
-text\<open>\<close>
-
-lemma E_sub_Earley_bin_list:
-  assumes "(k, cfg, inp, bs) \<in> wf_earley_input"
-  assumes "E_step k cfg inp (bins_items_upto bs k 0) \<subseteq> bins_items bs" "sound_items cfg inp (bins_items bs)"
-  assumes "is_sentence cfg inp" "nonempty_derives cfg"
-  shows "E k cfg inp (bins_items bs) \<subseteq> bins_items (Earley_bin_list k cfg inp bs)"
+lemma Earley_bin_sub_Earley_bin_list:
+  assumes "(k, cfg, \<omega>, bs) \<in> wf_earley_input"
+  assumes "sound_items cfg \<omega> (bins_items bs)"
+  assumes "is_sentence cfg \<omega>"
+  assumes "nonempty_derives cfg"
+  assumes "Earley_step k cfg \<omega> (bins_items_upto bs k 0) \<subseteq> bins_items bs"
+  shows "Earley_bin k cfg \<omega> (bins_items bs) \<subseteq> bins_items (Earley_bin_list k cfg \<omega> bs)"
 (*<*)
   sorry
 (*>*)
@@ -568,10 +452,10 @@ lemma E_sub_Earley_bin_list:
 text\<open>\<close>
 
 lemma Earley_sub_Earley_list:
-  assumes "k \<le> length \<omega>"
   assumes "wf_cfg cfg"
   assumes "is_sentence cfg \<omega>"
   assumes "nonempty_derives cfg"
+  assumes "k \<le> length \<omega>"
   shows "Earley k cfg \<omega> \<subseteq> bins_items (Earley_list k cfg \<omega>)"
 (*<*)
   sorry
